further rm next_epoch from ClientHist, leaving epochs_hist as the only updated field in the specs

src/program_proof/pav/client_hist.v
@@ -76,26 +76,26 @@ Record t :=
     (* epochs_hist allows stating the "intuitive" KT consistency property:
     that a client knows its key at every epoch. *)
     epochs_hist: list (option pk_ty);
-    next_epoch: w64;
     serv: Server.t;
     serv_is_good: bool;
   }.
 Global Instance eta : Settable _ :=
-  settable! mk <γ; uid; epochs_hist; next_epoch; serv; serv_is_good>.
+  settable! mk <γ; uid; epochs_hist; serv; serv_is_good>.
 
 Section defs.
 Context `{!heapGS Σ, !pavG Σ}.
 
 Definition own (ptr : loc) (obj : t) : iProp Σ :=
-  ∃ puts_hist,
-  "%Hlt_ep" ∷ ⌜ Z.of_nat $ length obj.(epochs_hist) <= uint.Z obj.(next_epoch) ⌝ ∗
+  ∃ puts_hist (next_epoch : w64),
+  (* this doesn't hold for Get ops, but those are intentionally not part
+  of the ClientHist api. *)
+  "%Heq_next_ep" ∷ ⌜ Z.of_nat $ length obj.(epochs_hist) = uint.Z next_epoch ⌝ ∗
   "%Hhist_reln" ∷ ⌜ hist_epochs_puts.reln obj.(epochs_hist) puts_hist ⌝ ∗
 
   "Hcli" ∷ Client.own ptr (Client.mk obj.(γ) obj.(uid)
-    (W64 $ length puts_hist) obj.(next_epoch) obj.(serv)
-    obj.(serv_is_good)) ∗
+    (W64 $ length puts_hist) next_epoch obj.(serv) obj.(serv_is_good)) ∗
   "#Hhist" ∷ is_hist obj.(γ) obj.(serv).(Server.vrf_pk) obj.(uid)
-    puts_hist (W64 $ length obj.(epochs_hist)).
+    puts_hist next_epoch.
 
 Lemma lookup_msv ptr_c c ep opt_pk γaudit aud_ep :
   c.(epochs_hist) !! (uint.nat ep) = Some opt_pk →
@@ -138,10 +138,11 @@ Lemma wp_ClientHist__Put ptr_c c sl_pk d0 (pk : list w8) :
         "Hcli" ∷ ClientHist.own ptr_c c
       else
         let new_c :=
-          set ClientHist.next_epoch (λ _, word.add ep (W64 1))
-          (set ClientHist.epochs_hist (λ x, x ++
+          set ClientHist.epochs_hist (λ x, x ++
             replicate (uint.nat ep - length x) (mjoin $ last x) ++
-            [Some pk]) c) in
+            [Some pk]) c in
+        "%Hlt_ep" ∷ ⌜ Z.of_nat $ length c.(ClientHist.epochs_hist) <
+          uint.Z ep + 1 ⌝ ∗
         "Hcli" ∷ ClientHist.own ptr_c new_c)
   }}}.
 Proof.
@@ -151,7 +152,8 @@ Proof.
   simpl. iIntros "*". iNamed 1.
   iApply "HΦ". iFrame "∗%".
   case_match; iNamed "Herr"; [by iFrame "∗#"|].
-  iExists (puts_hist ++ [(ep, pk)]).
+  iSplit; [word|].
+  iExists (puts_hist ++ [(ep, pk)]), (word.add ep (W64 1)).
   do 3 try iSplit; simpl in *.
   - rewrite !length_app length_replicate /=. word.
   - iPureIntro.
@@ -163,9 +165,7 @@ Proof.
     replace (W64 (_ + _)%nat) with
       (word.add (W64 $ length puts_hist) (W64 1)); [|word].
     iFrame.
-  - rewrite !length_app length_replicate /=.
-    iEval (replace (W64 _) with (word.add ep (W64 1)) by word).
-    iApply (hist_extend_put with "[$Hhist $His_put_post]"); word.
+  - iApply (hist_extend_put with "[$Hhist $His_put_post]"); word.
 Qed.
 
 Lemma wp_ClientHist__SelfMon ptr_c c :
@@ -183,9 +183,10 @@ Lemma wp_ClientHist__SelfMon ptr_c c :
         "Hcli" ∷ ClientHist.own ptr_c c
       else
         let new_c :=
-          set ClientHist.next_epoch (λ _, word.add ep (W64 1))
-          (set ClientHist.epochs_hist (λ x, x ++
-            replicate (uint.nat ep + 1 - length x) (mjoin $ last x)) c) in
+          set ClientHist.epochs_hist (λ x, x ++
+            replicate (uint.nat ep + 1 - length x) (mjoin $ last x)) c in
+        "%Hlt_ep" ∷ ⌜ Z.of_nat $ length c.(ClientHist.epochs_hist) <=
+          uint.Z ep + 1 ⌝ ∗
         "Hcli" ∷ ClientHist.own ptr_c new_c)
   }}}.
 Proof.
@@ -195,15 +196,16 @@ Proof.
   simpl. iIntros "*". iNamed 1.
   iApply "HΦ". iFrame "∗%".
   case_match; iNamed "Herr"; [by iFrame "∗#"|].
-  iExists puts_hist.
+  iSplit; [word|].
+  iExists puts_hist, (word.add ep (W64 1)).
   do 3 try iSplit; simpl in *.
   - rewrite !length_app length_replicate. word.
   - iPureIntro.
     by apply hist_epochs_puts.update_replicate.
   - iFrame.
-  - rewrite !length_app length_replicate.
-    iEval (replace (W64 _) with (word.add ep (W64 1)) by word).
-    iApply (hist_extend_selfmon with "[$Hhist $His_selfmon_post]"); word.
+  - iApply (hist_extend_selfmon with "[$Hhist $His_selfmon_post]"); word.
 Qed.
 
 End proof.
+
+Global Typeclasses Opaque ClientHist.own.
